Grinding through type soundness again
At least I think the invariant is correct now.

metatheory/typeSysPropsScript.sml
@@ -31,12 +31,6 @@ cases_on `keys` >>
 cases_on `vals` >>
 fs []);
 
-val tenv_ok_def = Define `
-(tenv_ok Empty = T) ∧
-(tenv_ok (Bind_tvar n tenv) = tenv_ok tenv) ∧
-(tenv_ok (Bind_name x tvs t tenv) = 
-  (check_freevars (tvs + num_tvs tenv) [] t ∧ tenv_ok tenv))`;
-
 (* Non exception constructors must be defined in the same module as the type
  * they construct *)
 val same_module_def = Define `
@@ -62,9 +56,6 @@ rw [tenvC_ok_def, merge_def, ALL_DISTINCT_APPEND] >>
 eq_tac >>
 rw [disjoint_env_def, DISJOINT_DEF, EXTENSION] >>
 metis_tac []);
-
-val tenvM_ok_def = Define `
-tenvM_ok tenvM = EVERY (\(mn,tenv). tenv_ok (bind_var_list2 tenv Empty)) tenvM`;
 
 val tenvC_ok_lookup = Q.store_thm ("tenvC_ok_lookup",
 `!tenvC cn tvs ts tn.
@@ -1784,14 +1775,6 @@ val tid_exn_to_tc_11 = Q.store_thm ("tid_exn_to_tc_11",
 cases_on `x` >>
 cases_on `y` >>
 rw [tid_exn_to_tc_def]);
-
-val restrict_tenvM_ok = Q.store_thm ("restrict_tenvM_ok",
-`!tenvM mns. tenvM_ok tenvM ⇒ tenvM_ok (restrict_tenvM tenvM mns)`,
- induct_on `tenvM` >>
- rw [tenvM_ok_def, restrict_tenvM_def] >>
- PairCases_on `h` >>
- fs [tenvM_ok_def, restrict_tenvM_def] >>
- rw []);
 
 val restrict_tenvC_ok_lem = Q.prove (
 `!tenvC cns. h0 ∉ set (MAP FST tenvC) ⇒ h0 ∉ set (MAP FST (restrict_tenvC tenvC cns))`,
