metatheory/typeSoundInvariantsScript.sml
@@ -20,16 +20,16 @@ val _ = type_abbrev( "tenvS" , ``: (num, t) env``);
 
 (* A value has a type *)
 (* The number is how many deBruijn type variables are bound in the context. *)
-(*val type_v : nat -> tenvM -> tenvC -> tenvS -> v -> t -> bool*)
+(*val type_v : nat -> tenvC -> tenvS -> v -> t -> bool*)
 
 (* A value environment has a corresponding type environment.  Since all of the
  * entries in the environment are values, and values have no free variables,
  * each entry in the environment can be typed in the empty environment (if at
  * all) *)
-(*val type_env : tenvM -> tenvC -> tenvS -> envE -> tenvE -> bool*)
+(*val type_env : tenvC -> tenvS -> envE -> tenvE -> bool*)
 
 (* The type of the store *)
-(*val type_s : tenvM -> tenvC -> tenvS -> store -> bool*)
+(*val type_s : tenvC -> tenvS -> store -> bool*)
 
 (* An evaluation context has the second type when its hole is filled with a
  * value of the first type. *)
@@ -37,19 +37,9 @@ val _ = type_abbrev( "tenvS" , ``: (num, t) env``);
  * This is only used for constructor contexts, because the value restriction 
  * ensures that no other contexts can be created under a let binding. *)
 (*val type_ctxt : nat -> tenvM -> tenvC -> tenvS -> tenvE -> ctxt_frame -> t -> t -> bool*)
-(*val type_ctxts : nat -> tenvM -> tenvC -> tenvS -> list ctxt -> t -> t -> bool*)
-(*val type_state : nat -> tenvM -> tenvC -> tenvS -> state -> t -> bool*)
+(*val type_ctxts : nat -> tenvC -> tenvS -> list ctxt -> t -> t -> bool*)
+(*val type_state : nat -> tenvC -> tenvS -> state -> t -> bool*)
 (*val context_invariant : nat -> list ctxt -> nat -> bool*)
-
-(*val restrict_tenvM : tenvM -> list modN -> tenvM*)
- val _ = Define `
- (restrict_tenvM [] mns = ([]))
-/\ (restrict_tenvM ((mn, tenv)::tenvM) mns =  
-(if MEM mn mns then
-    (mn, tenv)::restrict_tenvM tenvM mns
-  else
-    restrict_tenvM tenvM mns))`;
-
 
 (*val restrict_tenvC : tenvC -> list (id conN) -> tenvC*)
  val _ = Define `
@@ -59,7 +49,6 @@ val _ = type_abbrev( "tenvS" , ``: (num, t) env``);
     (cn, x)::restrict_tenvC tenvC cns
   else
     restrict_tenvC tenvC cns))`;
-
 
 
 (* Type programs without imposing signatures.  This is needed for the type
@@ -90,79 +79,95 @@ type_top_ignore_sig menv cenv tenv (Tmod mn spec ds) [(mn,tenv')] cenv' emp)`;
 (consistent_con_env _ _ = F)`;
 
 
-val _ = Hol_reln ` (! tvs menv cenv senv b.
+ val _ = Define `
+ 
+(tenv_ok Empty = T)
+/\
+(tenv_ok (Bind_tvar n tenv) = (tenv_ok tenv))
+/\
+(tenv_ok (Bind_name x tvs t tenv) =  
+(check_freevars (tvs + num_tvs tenv) [] t /\ tenv_ok tenv))`;
+
+
+val _ = Define `
+ (tenvM_ok tenvM = (EVERY (\ (mn,tenv) .  tenv_ok (bind_var_list2 tenv Empty)) tenvM))`;
+
+
+val _ = Hol_reln ` (! tvs cenv senv b.
 T
 ==>
-type_v tvs menv cenv senv (Litv (Bool b)) Tbool)
+type_v tvs cenv senv (Litv (Bool b)) Tbool)
 
-/\ (! tvs menv cenv senv n.
+/\ (! tvs cenv senv n.
 T
 ==>
-type_v tvs menv cenv senv (Litv (IntLit n)) Tint)
+type_v tvs cenv senv (Litv (IntLit n)) Tint)
 
-/\ (! tvs menv cenv senv.
+/\ (! tvs cenv senv.
 T
 ==>
-type_v tvs menv cenv senv (Litv Unit) Tunit)
+type_v tvs cenv senv (Litv Unit) Tunit)
 
-/\ (! tvs menv cenv senv cn vs tvs' tn ts' ts.
+/\ (! tvs cenv senv cn vs tvs' tn ts' ts.
 (EVERY (check_freevars tvs []) ts' /\
 ((LENGTH tvs' = LENGTH ts') /\
-(type_vs tvs menv cenv senv vs (MAP (type_subst (ZIP (tvs', ts'))) ts) /\
+(type_vs tvs cenv senv vs (MAP (type_subst (ZIP (tvs', ts'))) ts) /\
 (lookup cn cenv = SOME (tvs', ts, tn)))))
 ==>
-type_v tvs menv cenv senv (Conv (SOME cn) vs) (Tapp ts' (tid_exn_to_tc tn)))
+type_v tvs cenv senv (Conv (SOME cn) vs) (Tapp ts' (tid_exn_to_tc tn)))
 
-/\ (! tvs menv cenv senv vs ts.
-(type_vs tvs menv cenv senv vs ts)
+/\ (! tvs cenv senv vs ts.
+(type_vs tvs cenv senv vs ts)
 ==>
-type_v tvs menv cenv senv (Conv NONE vs) (Tapp ts TC_tup))
+type_v tvs cenv senv (Conv NONE vs) (Tapp ts TC_tup))
 
 /\ (! tvs menv cenv senv envC envM env tenv n e t1 t2.
 (consistent_con_env envC (restrict_tenvC cenv (MAP FST envC)) /\
-(consistent_mod_env senv (restrict_tenvC cenv (MAP FST envC)) envM (restrict_tenvM menv (MAP FST envM)) /\
-(type_env menv cenv senv env tenv /\
+(tenvM_ok menv /\
+(consistent_mod_env senv (restrict_tenvC cenv (MAP FST envC)) envM menv /\
+(type_env cenv senv env tenv /\
 (check_freevars tvs [] t1 /\
-type_e (restrict_tenvM menv (MAP FST envM)) (restrict_tenvC cenv (MAP FST envC)) (bind_tenv n( 0) t1 (bind_tvar tvs tenv)) e t2))))
+type_e menv (restrict_tenvC cenv (MAP FST envC)) (bind_tenv n( 0) t1 (bind_tvar tvs tenv)) e t2)))))
 ==>
-type_v tvs menv cenv senv (Closure (envM, envC, env) n e) (Tfn t1 t2))
+type_v tvs cenv senv (Closure (envM, envC, env) n e) (Tfn t1 t2))
 
 /\ (! tvs menv cenv senv envM envC env funs n t tenv tenv'.
 (consistent_con_env envC (restrict_tenvC cenv (MAP FST envC)) /\
-(consistent_mod_env senv (restrict_tenvC cenv (MAP FST envC)) envM (restrict_tenvM menv (MAP FST envM)) /\
-(type_env menv cenv senv env tenv /\
-(type_funs (restrict_tenvM menv (MAP FST envM)) (restrict_tenvC cenv (MAP FST envC)) (bind_var_list( 0) tenv' (bind_tvar tvs tenv)) funs tenv' /\
-(lookup n tenv' = SOME t)))))
+(tenvM_ok menv /\
+(consistent_mod_env senv (restrict_tenvC cenv (MAP FST envC)) envM menv /\
+(type_env cenv senv env tenv /\
+(type_funs menv (restrict_tenvC cenv (MAP FST envC)) (bind_var_list( 0) tenv' (bind_tvar tvs tenv)) funs tenv' /\
+(lookup n tenv' = SOME t))))))
 ==>
-type_v tvs menv cenv senv (Recclosure (envM, envC, env) funs n) t)
+type_v tvs cenv senv (Recclosure (envM, envC, env) funs n) t)
 
-/\ (! tvs menv cenv senv n t.
+/\ (! tvs cenv senv n t.
 (check_freevars( 0) [] t /\
 (lookup n senv = SOME t))
 ==>
-type_v tvs menv cenv senv (Loc n) (Tref t))
+type_v tvs cenv senv (Loc n) (Tref t))
 
-/\ (! tvs menv cenv senv.
+/\ (! tvs cenv senv.
 T
 ==>
-type_vs tvs menv cenv senv [] [])
+type_vs tvs cenv senv [] [])
 
-/\ (! tvs menv cenv senv v vs t ts.
-(type_v tvs menv cenv senv v t /\
-type_vs tvs menv cenv senv vs ts)
+/\ (! tvs cenv senv v vs t ts.
+(type_v tvs cenv senv v t /\
+type_vs tvs cenv senv vs ts)
 ==>
-type_vs tvs menv cenv senv (v::vs) (t::ts))
+type_vs tvs cenv senv (v::vs) (t::ts))
 
-/\ (! menv cenv senv.
+/\ (! cenv senv.
 T
 ==>
-type_env menv cenv senv emp Empty)
+type_env cenv senv emp Empty)
 
-/\ (! menv cenv senv n v env t tenv tvs.
-(type_v tvs menv cenv senv v t /\
-type_env menv cenv senv env tenv)
+/\ (! cenv senv n v env t tenv tvs.
+(type_v tvs cenv senv v t /\
+type_env cenv senv env tenv)
 ==>
-type_env menv cenv senv (bind n v env) (bind_tenv n tvs t tenv))
+type_env cenv senv (bind n v env) (bind_tenv n tvs t tenv))
 
 /\ (! tenvS tenvC.
 T
@@ -172,16 +177,16 @@ consistent_mod_env tenvS tenvC [] [])
 /\ (! tenvS tenvC mn env menv mn' tenv tenvM.
 ((mn = mn') /\
 (~ (MEM mn (MAP FST tenvM)) /\
-(type_env tenvM tenvC tenvS env (bind_var_list2 tenv Empty) /\
+(type_env tenvC tenvS env (bind_var_list2 tenv Empty) /\
 consistent_mod_env tenvS tenvC menv tenvM)))
 ==>
 consistent_mod_env tenvS tenvC ((mn,env)::menv) ((mn',tenv)::tenvM))`;
 
 val _ = Define `
- (type_s menv cenv senv s =  
+ (type_s cenv senv s =  
 (! l. 
     ((? t. lookup l senv = SOME t) <=> (? v. store_lookup l s = SOME v)) /\    
-(! t v. ((lookup l senv = SOME t) /\ (store_lookup l s = SOME v)) ==> type_v( 0) menv cenv senv v t)))`;
+(! t v. ((lookup l senv = SOME t) /\ (store_lookup l s = SOME v)) ==> type_v( 0) cenv senv v t)))`;
 
 
 val _ = Hol_reln ` (! n.
@@ -271,7 +276,7 @@ type_ctxt tvs menv cenv senv tenv (Capp1 op ()  e) t1 t3)
 /\ (! tvs menv cenv senv tenv op v t1 t2 t3.
 (check_freevars tvs [] t2 /\
 (check_freevars tvs [] t3 /\
-(type_v( 0) menv cenv senv v t1 /\
+(type_v( 0) cenv senv v t1 /\
 type_op op t1 t2 t3)))
 ==>
 type_ctxt tvs menv cenv senv tenv (Capp2 op v () ) t2 t3)
@@ -293,7 +298,7 @@ type_ctxt tvs menv cenv senv tenv (Cif ()  e1 e2) Tbool t)
    ALL_DISTINCT (pat_bindings p []) /\   
 (type_p tvs cenv p t1 tenv' /\
    type_e menv cenv (bind_var_list( 0) tenv' tenv) e t2)) /\
-type_v( 0) menv cenv senv err_v Texn))
+type_v( 0) cenv senv err_v Texn))
 ==>
 type_ctxt tvs menv cenv senv tenv (Cmat ()  pes err_v) t1 t2)
 
@@ -306,7 +311,7 @@ type_ctxt tvs menv cenv senv tenv (Clet n ()  e) t1 t2)
 /\ (! tvs menv cenv senv tenv cn vs es ts1 ts2 t tn ts' tvs'.
 (EVERY (check_freevars tvs []) ts' /\
 ((LENGTH tvs' = LENGTH ts') /\
-(type_vs tvs menv cenv senv (REVERSE vs)
+(type_vs tvs cenv senv (REVERSE vs)
         (MAP (type_subst (ZIP (tvs', ts'))) ts1) /\
 (type_es menv cenv (bind_tvar tvs tenv) es (MAP (type_subst (ZIP (tvs', ts'))) ts2) /\
 (lookup cn cenv = SOME (tvs', ((ts1++[t])++ts2), tn))))))
@@ -316,7 +321,7 @@ type_ctxt tvs menv cenv senv tenv (Ccon (SOME cn) vs ()  es) (type_subst (ZIP (t
 
 /\ (! tvs menv cenv senv tenv vs es t ts1 ts2.
 (check_freevars tvs [] t /\
-(type_vs tvs menv cenv senv (REVERSE vs) ts1 /\
+(type_vs tvs cenv senv (REVERSE vs) ts1 /\
 type_es menv cenv (bind_tvar tvs tenv) es ts2))
 ==>
 type_ctxt tvs menv cenv senv tenv (Ccon NONE vs ()  es) t (Tapp ((ts1++[t])++ts2) TC_tup))`;
@@ -339,41 +344,42 @@ val _ = Define `
   )))`;
 
 
-val _ = Hol_reln ` (! tvs tenvM tenvC senv t.
+val _ = Hol_reln ` (! tvs tenvC senv t.
 (check_freevars tvs [] t)
 ==>
-type_ctxts tvs tenvM tenvC senv [] t t)
+type_ctxts tvs tenvC senv [] t t)
 
 /\ (! tvs tenvM tenvC senv c envM envC env cs tenv t1 t2 t3.
-(type_env tenvM tenvC senv env tenv /\
+(type_env tenvC senv env tenv /\
 (consistent_con_env envC (restrict_tenvC tenvC (MAP FST envC)) /\
-(consistent_mod_env senv (restrict_tenvC tenvC (MAP FST envC)) envM (restrict_tenvM tenvM (MAP FST envM)) /\
-(type_ctxt tvs (restrict_tenvM tenvM (MAP FST envM)) (restrict_tenvC tenvC (MAP FST envC)) senv tenv c t1 t2 /\
-type_ctxts (if is_ccon c /\ poly_context cs then tvs else  0) tenvM tenvC senv cs t2 t3))))
+(tenvM_ok tenvM /\
+(consistent_mod_env senv (restrict_tenvC tenvC (MAP FST envC)) envM tenvM /\
+(type_ctxt tvs tenvM (restrict_tenvC tenvC (MAP FST envC)) senv tenv c t1 t2 /\
+type_ctxts (if is_ccon c /\ poly_context cs then tvs else  0) tenvC senv cs t2 t3)))))
 ==>
-type_ctxts tvs tenvM tenvC senv ((c,(envM,envC,env))::cs) t1 t3)`;
+type_ctxts tvs tenvC senv ((c,(envM,envC,env))::cs) t1 t3)`;
 
 val _ = Hol_reln ` (! dec_tvs tenvM tenvC senv envM envC s env e c t1 t2 tenv tvs.
 (context_invariant dec_tvs c tvs /\
 (consistent_con_env envC (restrict_tenvC tenvC (MAP FST envC)) /\
-(consistent_mod_env senv (restrict_tenvC tenvC (MAP FST envC)) envM (restrict_tenvM tenvM (MAP FST envM)) /\
-(type_ctxts tvs tenvM tenvC senv c t1 t2 /\
-(type_env tenvM tenvC senv env tenv /\
-(type_s tenvM tenvC senv s /\
-(type_e (restrict_tenvM tenvM (MAP FST envM)) (restrict_tenvC tenvC (MAP FST envC)) (bind_tvar tvs tenv) e t1 /\
-(( ~ (tvs =( 0))) ==> is_value e))))))))
+(tenvM_ok tenvM /\
+(consistent_mod_env senv (restrict_tenvC tenvC (MAP FST envC)) envM tenvM /\
+(type_ctxts tvs tenvC senv c t1 t2 /\
+(type_env tenvC senv env tenv /\
+(type_s tenvC senv s /\
+(type_e tenvM (restrict_tenvC tenvC (MAP FST envC)) (bind_tvar tvs tenv) e t1 /\
+(( ~ (tvs =( 0))) ==> is_value e)))))))))
 ==>
-type_state dec_tvs tenvM tenvC senv ((envM, envC, env), s, Exp e, c) t2)
+type_state dec_tvs tenvC senv ((envM, envC, env), s, Exp e, c) t2)
 
-/\ (! dec_tvs tenvM tenvC senv envM envC s env v c t1 t2 tenv tvs.
+/\ (! dec_tvs tenvC senv envM envC s env v c t1 t2 tenv tvs.
 (context_invariant dec_tvs c tvs /\
 (consistent_con_env envC (restrict_tenvC tenvC (MAP FST envC)) /\
-(consistent_mod_env senv (restrict_tenvC tenvC (MAP FST envC)) envM (restrict_tenvM tenvM (MAP FST envM)) /\
-(type_ctxts tvs tenvM tenvC senv c t1 t2 /\
-(type_env tenvM tenvC senv env tenv /\
-(type_s tenvM tenvC senv s /\
-type_v tvs tenvM tenvC senv v t1))))))
+(type_ctxts tvs tenvC senv c t1 t2 /\
+(type_env tenvC senv env tenv /\
+(type_s tenvC senv s /\
+type_v tvs tenvC senv v t1)))))
 ==>
-type_state dec_tvs tenvM tenvC senv ((envM, envC, env), s, Val v, c) t2)`;
+type_state dec_tvs tenvC senv ((envM, envC, env), s, Val v, c) t2)`;
 val _ = export_theory()
 
